start bottom up approach

Common.thy
@@ -10,10 +10,11 @@ fun toList :: "'a state \<Rightarrow> 'a list" where
   "toList (Idle current idle) = Current.toList current"
 | "toList (Copy current old new _) = Current.toList current"
 
+(* TODO: unnecessary function *)
 fun normalize :: "'a state \<Rightarrow> 'a state" where
   "normalize (Copy current old new moved) = (
       case current of Current extra added _ remained \<Rightarrow> 
-      if moved = remained
+      if moved \<ge> remained
       then Idle current (idle.Idle (Stack extra new) (added + moved))
       else Copy current old new moved
   )"
@@ -37,10 +38,28 @@ fun pop :: "'a state \<Rightarrow> 'a * 'a state" where
   "pop (Idle current (idle.Idle stack stackSize)) = 
       (top current, Idle (bottom current) (idle.Idle (Stack.pop stack) (stackSize - 1)))"
 | "pop (Copy current aux new moved) = 
-      (top current, Copy (bottom current) aux new moved)"
+      (top current, normalize (Copy (bottom current) aux new moved))"
 
 fun isEmpty :: "'a state \<Rightarrow> bool" where
   "isEmpty (Idle current _) = Current.isEmpty current"
 | "isEmpty (Copy current _ _ _) = Current.isEmpty current"
+
+fun invariant :: "'a state \<Rightarrow> bool" where
+  "invariant (Idle current idle) \<longleftrightarrow> 
+     Current.toList current = Idle.toList idle 
+   \<and> Idle.invariant idle
+   \<and> Current.invariant current"
+| "invariant (Copy current aux new moved) \<longleftrightarrow> (
+    case current of Current _ _ old remained \<Rightarrow>
+    let aux = take (remained - moved) aux in
+      Stack.toList old = rev aux @ new
+    \<and> moved < remained
+    \<and> moved = List.length new
+    \<and> Current.invariant current
+ )"
+
+fun remainingSteps :: "'a state \<Rightarrow> nat" where
+  "remainingSteps (Idle current idle) = 0"
+| "remainingSteps (Copy (Current _ _ _ remained) aux new moved) = remained - moved"
 
 end
