Idle.thy
@@ -7,4 +7,16 @@ datatype 'a idle = Idle "'a stack" nat
 fun toList :: "'a idle \<Rightarrow> 'a list" where
   "toList (Idle stack _) = Stack.toList stack"
 
+fun push :: "'a \<Rightarrow> 'a idle \<Rightarrow> 'a idle" where
+  "push x (Idle stack stackSize) = Idle (Stack.push x stack) (Suc stackSize)"
+
+fun pop :: "'a idle \<Rightarrow> ('a * 'a idle)" where
+  "pop (Idle stack stackSize) = (Stack.first stack, Idle (Stack.pop stack) (stackSize - 1))"
+
+fun size :: "'a idle \<Rightarrow> nat" where
+  "size (Idle _ stackSize) = stackSize"
+
+fun invariant :: "'a idle \<Rightarrow> bool" where
+  "invariant (Idle stack stackSize) \<longleftrightarrow> Stack.size stack = stackSize"
+  
 end
