RealTimeDeque_Proof.thy
@@ -1,23 +1,179 @@
 theory RealTimeDeque_Proof
-  imports Deque RealTimeDeque Transformation_Proof 
+  imports Deque RealTimeDeque Idle_Proof Transformation_Proof
 begin
 
-(* TODO: Stricter invariant!
-lemma please_1: "\<lbrakk>RealTimeDeque.invariant (Transforming (transformation.Left left right));
-      ticksHelper (right, left) =  (Big.state.Common (state.Idle x21a (idle.Idle x1d x2d)), Small.state.Common (state.Idle x21 (idle.Idle x1c x2c)))\<rbrakk>
-       \<Longrightarrow> Stack.toList x1c @ rev (Stack.toList x1d) = Small.toList left @ rev (Current.toList x21a)"
-  apply(induction "Transforming (transformation.Left left right)" rule: RealTimeDeque.invariant.induct)
-  apply(auto split: if_splits current.splits)
+fun t_invariant_1' :: "'a transformation \<Rightarrow> bool" where
+  "t_invariant_1' (Left left right) = (
+  \<exists>n currentL idleL nL currentR idleR nR. 
+  nTicks n (Left left right) = 
+    Left (Small.state.Common (state.Idle currentL (idle.Idle idleL nL))) 
+         (Big.state.Common   (state.Idle currentR (idle.Idle idleR nR)))
+  \<and> Small.toList left @ rev (Big.toList right) = Stack.toList idleL @ rev (Stack.toList idleR)
+  \<and> Stack.toList idleL @ rev (Stack.toList idleR) = Current.toList currentL @ rev (Current.toList currentR)
+  )"
+| "t_invariant_1' (Right left right) = True"
+
+fun t_invariant_1 :: "'a transformation \<Rightarrow> bool" where
+  "t_invariant_1 (Left left right) = (
+    case fourTicks (Left left right) of 
+      (Left (Small.state.Common (state.Idle currentL (idle.Idle idleL _))) 
+            (Big.state.Common   (state.Idle currentR (idle.Idle idleR _)))) \<Rightarrow>
+      Small.toList left @ rev (Big.toList right) = Stack.toList idleL @ rev (Stack.toList idleR) \<and>
+      Current.toList currentL @ rev (Current.toList currentR) = Stack.toList idleL @ rev (Stack.toList idleR)
+    | _ \<Rightarrow> True
+  )"
+| "t_invariant_1 (Right left right) = True"
+
+lemma "t_invariant_1' t \<Longrightarrow> t_invariant_1 t"
+  apply(induction t)
+   apply(auto split: prod.splits state_splits)
   sorry
 
+fun t_invariant :: "'a transformation \<Rightarrow> bool" where
+  "t_invariant (Left left right) = (\<forall>x.
+    case fourTicks (Left (push x left) right) of 
+      (Left (Small.state.Common (state.Idle currentL (idle.Idle idleL _))) 
+            (Big.state.Common   (state.Idle currentR (idle.Idle idleR _)))) \<Rightarrow>
+      x # Small.toList left @ rev (Big.toList right) = Stack.toList idleL @ rev (Stack.toList idleR) \<and>
+      Current.toList currentL @ rev (Current.toList currentR) = Stack.toList idleL @ rev (Stack.toList idleR)
+    | _ \<Rightarrow> True
+  )"
+| "t_invariant (Right left right) = True"
 
-lemma please: "\<lbrakk>RealTimeDeque.invariant (Transforming (transformation.Left left right));
-        ticksHelper (x1b, x2b) = (Big.state.Common (state.Idle x21a (idle.Idle x1d x2d)), Small.state.Common (state.Idle x21 (idle.Idle x1c x2c)));
-        ticksHelper (x1a, x2a) = (x1b, x2b); ticksHelper (x1, x2) = (x1a, x2a); ticksHelper (right, left) = (x1, x2)\<rbrakk>
-       \<Longrightarrow> Stack.toList x1c @ rev (Stack.toList x1d) = Small.toList left @ rev (Current.toList x21a)"
-  apply(induction "(right, left)" rule: ticksHelper.induct)
-  apply(auto split: current.splits)
-  sorry *)
+lemma "t_invariant_1' t = t_invariant_1' (ticks t)"
+  apply(induction t)
+   apply(auto split: prod.splits)
+  sorry
+
+fun runningFold :: "('a deque \<Rightarrow> 'a deque) list \<Rightarrow> 'a deque \<Rightarrow> 'a deque list" where
+  "runningFold [] _ = []"
+| "runningFold (x#xs) deque = (
+  let deque = x deque 
+  in deque # runningFold xs deque
+)"
+
+value "runningFold 
+  [
+  enqueueLeft (0::int), 
+  enqueueLeft 1, 
+  enqueueLeft 2,
+  enqueueLeft 3,
+  enqueueLeft 4,
+  enqueueLeft 5,
+  enqueueLeft 6,
+  enqueueLeft 7,
+  enqueueLeft 8,
+  enqueueLeft 9,
+  enqueueLeft 10,
+  enqueueLeft 11,
+  enqueueLeft 12,
+  enqueueLeft 13,
+  enqueueLeft 14,
+  enqueueLeft 15,  
+  enqueueLeft 16,
+  enqueueLeft 17,
+  enqueueLeft 18,
+  enqueueLeft 19,
+  enqueueLeft 20,
+  dequeueLeft,
+  dequeueLeft,
+  dequeueLeft,
+  dequeueLeft,
+  dequeueLeft
+  ] 
+  Empty"
+
+fun invariant :: "'a deque \<Rightarrow> bool" where
+  "invariant Empty = True"
+| "invariant (One _) = True"
+| "invariant (Two _ _) = True"
+| "invariant (Three _ _ _) = True"
+| "invariant (Idle (idle.Idle left leftLength) (idle.Idle right rightLength)) = (
+   Stack.size left = leftLength \<and>
+   Stack.size right = rightLength \<and>
+   (leftLength \<ge> 2 \<or> rightLength \<ge> 2)
+  )"
+| "invariant (Transforming (Left left right)) = (\<forall>x.
+    case fourTicks (Left (push x left) right) of 
+      (Left (Small.state.Common (state.Idle currentL (idle.Idle idleL _))) 
+            (Big.state.Common   (state.Idle currentR (idle.Idle idleR _)))) \<Rightarrow>
+      x # Small.toList left @ rev (Big.toList right) = Stack.toList idleL @ rev (Stack.toList idleR) \<and>
+      Current.toList currentL @ rev (Current.toList currentR) = Stack.toList idleL @ rev (Stack.toList idleR)
+    | _ \<Rightarrow> True
+  )"
+| "invariant (Transforming (Right left right)) = (\<forall>x.
+    case fourTicks (Right (Big.push x left) right) of 
+      (Right (Big.state.Common   (state.Idle currentL (idle.Idle idleL _))) 
+             (Small.state.Common (state.Idle currentR (idle.Idle idleR _)))) \<Rightarrow>
+      x # Big.toList left @ rev (Small.toList right) = Stack.toList idleL @ rev (Stack.toList idleR) \<and>
+      Current.toList currentL @ rev (Current.toList currentR) = Stack.toList idleL @ rev (Stack.toList idleR)
+    | _ \<Rightarrow> True
+  )"
+
+(* TODO: Probably more strict needed! *)
+fun isIdle :: "'a transformation \<Rightarrow> bool" where
+  "isIdle (
+    Left 
+      (Small.state.Common (state.Idle currentL (idle.Idle idleL _))) 
+      (Big.state.Common   (state.Idle currentR (idle.Idle idleR _)))
+    ) = True"
+| "isIdle (
+    Right
+      (Big.state.Common   (state.Idle currentL (idle.Idle idleL _))) 
+      (Small.state.Common (state.Idle currentR (idle.Idle idleR _)))
+    ) = True"
+| "isIdle _ = False"
+
+fun invariant_t :: "'a deque \<Rightarrow> bool" where
+  "invariant_t Empty = True"
+| "invariant_t (One _) = True"
+| "invariant_t (Two _ _) = True"
+| "invariant_t (Three _ _ _) = True"
+| "invariant_t (Idle (idle.Idle left leftLength) (idle.Idle right rightLength)) = (
+   Stack.size left = leftLength \<and>
+   Stack.size right = rightLength \<and>
+   (leftLength \<ge> 2 \<or> rightLength \<ge> 2)
+  )"
+| "invariant_t (Transforming transformation) = (
+    let ticked = fourTicks transformation in
+    let steps = remainingSteps transformation in
+    let steps' = remainingSteps ticked in
+    steps - steps' = 4 \<or> 
+    (steps' = 0 \<and> isIdle ticked)
+  )"
+                     
+
+lemma ticks_inv: "\<lbrakk>
+  invariant_t (Transforming transformation)
+\<rbrakk> \<Longrightarrow> invariant_t (Transforming (fourTicks transformation))"
+  sorry
+
+value "Left (Reverse1 (Current [] 0 (Stack [] []) 0) (Stack [] []) []) (Reverse (Current [] 0 (Stack [] []) 2) (Stack [a\<^sub>1] [a\<^sub>1]) [] 2)"
+
+value "fourTicks ( (Left (Reverse1 (Current [] 0 (Stack [] []) 0) (Stack [] []) []) (Reverse (Current [] 0 (Stack [] []) 2) (Stack [a\<^sub>1] [a\<^sub>1]) [] 2)))"
+
+value "invariant_t (Transforming (Left (Reverse1 (Current [] 0 (Stack [] []) 0) (Stack [] []) []) (Reverse (Current [] 0 (Stack [] []) 2) (Stack [0::nat] [1]) [] 2)))"
+
+value "invariant_t (Transforming (ticks (Left (Reverse1 (Current [] 0 (Stack [] []) 0) (Stack [] []) []) (Reverse (Current [] 0 (Stack [] []) 2) (Stack [a\<^sub>1] [a\<^sub>1]) [] 2))))"
+
+
+lemma ticksLength: "Transformation.length t = Transformation.length (ticks t)"
+  by (simp add: ticks)
+
+lemma sixTicks_inv: 
+  assumes 
+    "invariant (Transforming (Right left right))" 
+  shows
+   "invariant (Transforming (sixTicks (Right left right)))"
+  sorry
+
+lemma helper: " \<lbrakk>
+  \<not> Suc (Stack.size left) \<le> 3 * Stack.size right;
+  leftLength = Stack.size left; 
+  rightLength = Stack.size right;
+  2 \<le> Stack.size left
+\<rbrakk> \<Longrightarrow> 3 * List.length (Stack.toList right) < Suc (List.length (Stack.toList (Stack.push x left)))"
+  by (simp add: Stack_Proof.push size_listLength)
 
 interpretation RealTimeDeque: Deque where
   empty    = empty    and
@@ -56,29 +212,32 @@ next
     case (Idle left right)
     then show ?case
     proof(induction x "Idle left right" rule: enqueueLeft.induct)
-      case (5 x left leftLength right rightLength)
+      case (5 x rightIdle rightLength)
       then show ?case 
-        by (auto simp: Stack_Proof.push Let_def all_ticks ticks_helper split: prod.splits)
+        apply (auto simp: Idle_Proof.push Let_def all_ticks ticks_helper split: prod.splits idle.splits)
+        (* TODO: *)
+        apply (metis Idle.toList.simps Idle_Proof.push)
+        by (metis Big.toList.simps(2) Current.toList.simps Idle.toList.simps Idle_Proof.push Small.toList.simps(2) append_Cons append_self_conv2 ticks_help ticks_help2)
     qed
   next
     case (Transforming t x)
     then show ?case 
-    proof(induction t arbitrary: x)
+    proof(induction t)
       case (Left left right)
       then show ?case 
-        apply(auto simp: Let_def ticks_help ticks_help2 small_push
-                  split: prod.splits Small.state.splits state_splits)
-        sorry
+        apply(auto simp: Let_def ticks_help ticks_help2 ticks_helpFUCK split: prod.splits state_splits)
+        by fastforce
     next
       case (Right left right)
       then show ?case
-         apply(auto simp: Let_def ticks_help ticks_help2 split: prod.splits state_splits)
-        sorry
+        apply(auto simp: Let_def ticks_help ticks_help2 ticks_helpFUCK' split: prod.splits state_splits)
+        by fastforce
     qed
   qed
 next
 case (4 q x)
-  then show ?case  sorry
+  then show ?case
+    sorry
 next
   case (5 q)
   then show ?case sorry
@@ -93,16 +252,144 @@ next
   then show ?case sorry
 next
   case (9 q)
-  then show ?case sorry
+  then show ?case 
+    sorry
 next
   case (10 q)
   then show ?case sorry
 next
   case 11
-  then show ?case sorry
+  then show ?case 
+    by (simp add: RealTimeDeque.empty_def)
 next
   case (12 q x)
-  then show ?case sorry
+  then show ?case
+  proof(induction x q rule: enqueueLeft.induct)
+  case (1 x)
+    then show ?case by auto
+  next
+    case (2 x y)
+    then show ?case by auto
+  next
+    case (3 x y z)
+    then show ?case by auto
+  next
+    case (4 x a b c)
+    then show ?case by auto 
+  next
+    case (5 x left right rightLength)
+    obtain left' leftLength where "idle.Idle left' leftLength = left"
+      apply(induction left)
+      by auto
+    
+    with 5 show ?case 
+    proof(induction "3 * rightLength \<ge> (Suc leftLength)")
+      case True
+      then show ?case
+        by(auto simp: Let_def size_push Stack_Proof.size_push split: prod.splits state_splits)
+    next
+      case False
+      let ?newDeque = "enqueueLeft x (deque.Idle left  (idle.Idle right rightLength))"
+      let ?pushedLeft = "Stack.push x left'"
+      let ?leftStart = "Reverse (Current [] 0 ?pushedLeft (leftLength - rightLength - 1)) ?pushedLeft [] (leftLength - rightLength - 1)"
+      let ?rightStart = "Reverse1 (Current [] 0 right (2 * rightLength + 1)) right []"
+      let ?transformationStart = "Right ?leftStart ?rightStart"
+
+      let ?newleftLength = "Big.length ?leftStart"
+      let ?newRightLength = "Small.length ?rightStart"    
+
+      from False.hyps False.prems have initialLength_same: "3 * ?newRightLength < Suc ?newleftLength"
+        by(auto simp: helper)
+
+      with False.prems False.hyps have "invariant (Transforming ?transformationStart)"
+        sorry
+
+      with False.prems sixTicks_inv have "invariant (Transforming (sixTicks ?transformationStart))"
+        using sixTicks_inv
+        by blast
+      
+      with False show ?case 
+        apply(auto simp: Stack_Proof.size_push Let_def size_push split: prod.splits state_splits)
+        sorry
+    qed
+    (*proof(induction left arbitrary: x)
+      case (Stack left1 left2)
+      then show ?case
+      proof(induction right arbitrary: x)
+        case (Stack right1 right2)
+        let ?newDeque = "enqueueLeft  x (deque.Idle (idle.Idle (Stack left1 left2) leftLength) (idle.Idle (Stack right1 right2) rightLength))"
+
+        have leftLength:  "leftLength = length left1 + length left2"
+          using Stack.prems
+          by auto
+        have rightLength: "rightLength = length right1 + length right2"
+          using Stack.prems
+          by auto
+     
+        from Stack.prems show ?case
+        proof(induction ?newDeque)
+          case Empty
+          then show ?case by auto
+        next
+          case (One a)
+          then show ?case
+            by(auto simp: Let_def)
+        next
+          case (Two a b)
+          then show ?case
+            by(auto simp: Let_def)
+        next
+          case (Three x1 x2a x3)
+          then show ?case 
+            by(auto simp: Let_def)
+        next
+          case (Idle newLeft newRight)
+          then show ?case 
+            by(auto simp: Let_def)
+        next
+          case (Transforming transformation)
+          then show ?case
+          proof(induction transformation)
+            case (Left newLeft newRight)
+            then show ?case
+              by (auto simp: Let_def split: prod.splits)
+          next
+            case (Right newLeft newRight)
+            with Right.prems show ?case
+            proof(cases "fourTicks (Right (Big.push x newLeft) newRight)")
+              case (Left leftInv rightInv)
+              then show ?thesis
+                by(auto simp: Let_def split: prod.splits)
+            next
+              case (Right leftInv rightInv)
+              from Right.prems show ?thesis
+              proof(induction "Suc (length left1 + length left2) \<le> 3 * length right1 + 3 * length right2")
+                case True
+                then show ?case by auto
+              next
+                case False
+
+             
+                from False.prems  have "invariant (Transforming (transformation.Right newLeft newRight))"
+                  apply(auto simp: Let_def split: prod.splits state_splits)
+                  sorry
+
+            
+                with False.prems show ?case
+                  by auto
+              qed       
+              qed
+             qed 
+            qed
+          qed
+        qed   *)
+  next
+    case (6 x left right)
+    then show ?case sorry
+  next
+    case (7 x left right)
+    then show ?case sorry
+  qed
 next
   case (13 q x)
   then show ?case sorry
@@ -112,6 +399,35 @@ next
 next
   case (15 q)
   then show ?case sorry
+next 
+  case (16 q)
+  then show ?case
+  proof(induction q)
+    case Empty
+    then show ?case by auto
+  next
+    case (One x)
+    then show ?case by auto
+  next
+    case (Two x1 x2a)
+    then show ?case by auto
+  next
+    case (Three x1 x2a x3)
+    then show ?case by auto
+  next
+    case (Idle x1 x2a)
+    then show ?case by auto
+  next
+    case (Transforming x)
+    then show ?case 
+    proof(induction x)
+      case (Left x1 x2)
+      then show ?case by auto
+    next
+      case (Right x1 x2)
+      then show ?case by auto
+      qed
+  qed
 qed
 
 end
