Small.thy
@@ -25,6 +25,8 @@ fun tick :: "'a state \<Rightarrow> 'a state" where
     else Reverse2 current auxS (Stack.pop big) ((first big)#newS) (count + 1)
   )"
 
+value "tick (Reverse2 (Current [] 0 (Stack [] [a\<^sub>1]) 1) [a\<^sub>1] (Stack [] []) [a\<^sub>2] 1)"
+
 fun push :: "'a \<Rightarrow> 'a state \<Rightarrow> 'a state" where
   "push x (Common state) = Common (Common.push x state)"
 | "push x (Reverse1 current small auxS) = Reverse1 (put x current) small auxS"
@@ -39,5 +41,42 @@ fun pop :: "'a state \<Rightarrow> 'a * 'a state" where
     (top current, Reverse1 (bottom current) small auxS)"
 | "pop (Reverse2 current auxS big newS count) = 
     (top current, Reverse2 (bottom current) auxS big newS count)"
+
+(* Just for proof *)
+fun length :: "'a state \<Rightarrow> nat" where
+  "length small = List.length (toList small)"
+
+fun isEmpty :: "'a state \<Rightarrow> bool" where
+  "isEmpty (Common state) = Common.isEmpty state"
+| "isEmpty (Reverse1 current _ _) = Current.isEmpty current"
+| "isEmpty (Reverse2 current _ _ _ _) = Current.isEmpty current"
+
+(* TODO: *)
+fun invariant :: "'a state \<Rightarrow> bool" where
+  "invariant (Common state) = Common.invariant state"
+| "invariant (Reverse1 current small auxS) = (
+   case current of Current _ _ old remained \<Rightarrow>
+   let smallSize = Stack.size small in
+      drop (remained - smallSize) (Stack.toList old) = drop (smallSize - remained) (Stack.toList small)
+    \<and> Stack.toList old = drop ((List.length auxS + smallSize) - remained) (rev auxS @ Stack.toList small)
+    \<and> remained > Stack.size old
+  )"
+| "invariant (Reverse2 current auxS big newS count) = (
+   case current of Current _ _ old remained \<Rightarrow>
+       Stack.toList old = drop (List.length auxS - remained) (rev auxS)
+    \<and> remained > Stack.size old
+    \<and> remained \<ge> count + Stack.size big
+    \<and> count = List.length newS
+)"
+
+fun pop_invariant :: "'a state \<Rightarrow> bool" where
+  "pop_invariant (Common state) = True"
+| "pop_invariant (Reverse1 current _ _) \<longleftrightarrow> True"
+| "pop_invariant (Reverse2 (Current _ _ _ remained) _ _ _ count) \<longleftrightarrow> remained > count"
+
+fun remainingSteps :: "'a state \<Rightarrow> nat" where
+  "remainingSteps (Common state) = Common.remainingSteps state"
+| "remainingSteps (Reverse1 _ small _) = Stack.size small"
+| "remainingSteps (Reverse2 _ _ big _ _) = Stack.size big"
 
 end
