Transformation.thy
@@ -2,10 +2,10 @@ theory Transformation
   imports Big Small
 begin
 
-fun ticksHelper :: "('a Big.state * 'a Small.state) \<Rightarrow> 'a Big.state * 'a Small.state" where
-  "ticksHelper (Reverse currentB big auxB 0, Reverse1 currentS _ auxS) =
-    (Big.Common (normalize (Copy currentB auxB [] 0)), Reverse2 currentS auxS big [] 0)"
-| "ticksHelper (left, right) = (Big.tick left, Small.tick right)"
+fun tickStates :: "('a Big.state * 'a Small.state) \<Rightarrow> 'a Big.state * 'a Small.state" where
+  "tickStates (Reverse currentB big auxB 0, Reverse1 currentS _ auxS) =
+    (Big.tick (Reverse currentB big auxB 0), Reverse2 currentS auxS big [] 0)"
+| "tickStates (left, right) = (Big.tick left, Small.tick right)"
 
 datatype 'a transformation =
    Left "'a Small.state" "'a Big.state"
@@ -14,14 +14,17 @@ datatype 'a transformation =
 fun toListLeft :: "'a transformation \<Rightarrow> 'a list" where
   "toListLeft (Left small big)  = Small.toList small  @ (rev (Big.toList big))"
 | "toListLeft (Right big small) = Big.toList big @ (rev (Small.toList small))"
+
+fun length :: "'a transformation \<Rightarrow> nat" where
+  "length transformation = List.length (toListLeft transformation)"
  
 fun toListRight :: "'a transformation \<Rightarrow> 'a list" where
   "toListRight (Left small big)  = Big.toList big @ (rev (Small.toList small))"
 | "toListRight (Right big small) = Small.toList small @ (rev (Big.toList big))"
 
 fun ticks :: "'a transformation \<Rightarrow> 'a transformation" where
-  "ticks (Left small big) = (case ticksHelper (big, small) of (big, small) \<Rightarrow> Left small big)"
-| "ticks (Right big small) = (case ticksHelper (big, small) of (big, small) \<Rightarrow> Right big small)"  
+  "ticks (Left small big) = (case tickStates (big, small) of (big, small) \<Rightarrow> Left small big)"
+| "ticks (Right big small) = (case tickStates (big, small) of (big, small) \<Rightarrow> Right big small)"  
 
 fun fourTicks where
   "fourTicks transformation = (ticks (ticks (ticks (ticks transformation))))"
@@ -29,5 +32,22 @@ fun fourTicks where
 fun sixTicks where
   "sixTicks transformation = ticks (ticks (fourTicks transformation))"
 
+fun nTicks :: "nat \<Rightarrow> 'a transformation \<Rightarrow> 'a transformation" where
+  "nTicks 0 transformation = transformation"
+| "nTicks (Suc n) transformation = nTicks n (ticks transformation)"
+
+fun remainingSteps :: "'a transformation \<Rightarrow> nat" where
+  "remainingSteps (Left small big) = max (Small.remainingSteps small) (Big.remainingSteps big)"
+| "remainingSteps (Right big small) = max (Small.remainingSteps small) (Big.remainingSteps big)"
+
+fun invariant :: "'a transformation \<Rightarrow> bool" where
+  "invariant (Left small big) = True"
+| "invariant (Right big small) = True"
+
+lemma fourTicks: "fourTicks t = nTicks 4 t"
+  by (simp add: numeral_Bit0)
+
+lemma sixTicks: "sixTicks t = nTicks 6 t"
+  by (metis add_One_commute add_Suc eval_nat_numeral(3) fourTicks fourTicks.simps nTicks.simps(2) numeral_plus_numeral semiring_norm(3) semiring_norm(4) sixTicks.simps)
 
 end
