Big_Proof.thy
@@ -2,8 +2,107 @@ theory Big_Proof
   imports Big Common_Proof
 begin
 
+lemma helper: "Big.toList (Big.tick (Reverse x1 x2a x3 x4)) = Current.toList x1"
+  apply(induction x4)
+  by(auto split: current.splits)
+
 lemma tick: "toList (tick state) = toList state"
   apply(induction state)
-  by(auto simp: tick)
+  by(auto simp: helper tick)
+
+lemma helper_1: "tick (Reverse current big auxB count) = Reverse current' big' auxB' count' 
+            \<Longrightarrow> Current.invariant current 
+            \<Longrightarrow> Current.invariant current'"
+  apply(induction "(Reverse current big auxB count)" arbitrary: big auxB count big' auxB' count' rule: tick.induct)
+  by auto
+
+lemma invariant_tick: "invariant state \<Longrightarrow> invariant (tick state)"
+  apply(induction state rule: tick.induct)
+    apply(auto simp: rev_take invariant_tick split: current.splits)
+  (* TODO: *)
+  by (smt (z3) Nat.diff_diff_right Stack_Proof.pop Suc_le_D add_Suc_right append_Nil2 diff_diff_cancel diff_less empty first length_drop length_rev nat_less_le size_listLength take_Nil take_Suc zero_less_Suc)
+
+lemma pop: "\<lbrakk>\<not> isEmpty big; pop big = (x, big')\<rbrakk> \<Longrightarrow> x # toList big' = toList big"
+  apply(induction big arbitrary: x rule: pop.induct)
+  by(auto simp: get Common_Proof.pop split: prod.splits current.splits if_splits)
+
+lemma push: "toList (push x big) = x # toList big"
+  apply(induction x big rule: push.induct)
+  by(auto simp: put Common_Proof.push)
+
+lemma invariant_push: "invariant big \<Longrightarrow> invariant (push x big)"
+proof(induction x big rule: push.induct)
+  case (1 x state)
+  then show ?case by(auto simp: invariant_push)
+next
+  case (2 x current big auxB count)
+  then show ?case by(auto split: current.splits)
+qed
+
+lemma helper_2: "\<lbrakk>
+  current = Current x1 (List.length x1) x3 (Stack.size x3); count < Stack.size x3;
+  \<not> Current.isEmpty (Current x1 (List.length x1) x3 (Stack.size x3));
+  Stack.toList x3 = drop (List.length auxB + count - Stack.size x3) (rev auxB) @ take count (Stack.toList big);
+  Stack.size x3 - count \<le> List.length auxB; 
+  get (Current x1 (List.length x1) x3 (Stack.size x3)) = (x, Current x1a x2a x3a x4);
+  big' = Reverse (Current x1a x2a x3a x4) big auxB count\<rbrakk>
+       \<Longrightarrow> Stack.toList x3a = drop (List.length auxB + count - x4) (rev auxB) @ drop (count - x4) (take count (Stack.toList big))"
+proof(induction "Current x1 (List.length x1) x3 (Stack.size x3)" rule: get.induct)
+  case 1
+  then show ?case 
+    apply auto
+    (* TODO *)
+    by (smt (z3) Nat.diff_diff_right Stack_Proof.pop Suc_diff_Suc Suc_diff_le diff_diff_cancel diff_is_0_eq helper_2 leD le_diff_conv length_0_conv length_drop length_rev less_imp_le not_less_eq rev_take tl_append2)
+next
+  case (2 x xs)
+  then show ?case by auto
+qed
+
+lemma helper_3: "\<lbrakk>current = Current x1 (List.length x1) x3 (Stack.size x3); count < Stack.size x3;
+        \<not> Current.isEmpty (Current x1 (List.length x1) x3 (Stack.size x3));
+        Stack.toList x3 = drop (List.length auxB + count - Stack.size x3) (rev auxB) @ take count (Stack.toList big);
+        Stack.size x3 - count \<le> List.length auxB; get (Current x1 (List.length x1) x3 (Stack.size x3)) = (x, Current x1a x2a x3a x4);
+        big' = Reverse (Current x1a x2a x3a x4) big auxB count\<rbrakk>
+       \<Longrightarrow> x4 - count \<le> List.length auxB"
+proof(induction "Current x1 (List.length x1) x3 (Stack.size x3)" rule: get.induct)
+  case 1
+then show ?case by auto
+next
+  case (2 x xs)
+  then show ?case by auto
+qed
+
+lemma helper_4: "\<lbrakk>
+  current = Current x1 (List.length x1) x3 (Stack.size x3);
+  count < Stack.size x3;
+  \<not> Current.isEmpty (Current x1 (List.length x1) x3 (Stack.size x3));
+  Stack.toList x3 = drop (List.length auxB + count - Stack.size x3) (rev auxB) @ take count (Stack.toList big);
+  Stack.size x3 - count \<le> List.length auxB; get (Current x1 (List.length x1) x3 (Stack.size x3)) = (x, Current x1a x2a x3a x4);
+  big' = Reverse (Current x1a x2a x3a x4) big auxB count
+\<rbrakk> \<Longrightarrow> count \<le> x4"
+proof(induction "Current x1 (List.length x1) x3 (Stack.size x3)" rule: get.induct)
+case 1
+  then show ?case by auto
+next
+  case (2 x xs)
+  then show ?case by auto
+qed
+
+lemma invariant_pop: "\<lbrakk>\<not> isEmpty big; invariant big; pop_invariant big; pop big = (x, big')\<rbrakk>
+   \<Longrightarrow> invariant big'"
+proof(induction big arbitrary: x rule: pop.induct)
+  case (1 state)
+  then show ?case
+    by(auto simp: Common_Proof.invariant_pop split: prod.splits)
+next
+  case (2 current big auxB count)
+  then show ?case
+    apply(auto split: current.splits prod.splits)
+  (* TODO: *)
+    apply (meson Big_Proof.helper_2)
+       apply (meson Current.invariant.simps invariant_get)+
+     apply (meson helper_3)
+    by (meson helper_4)
+qed
 
 end
