Common_Proof.thy
@@ -11,10 +11,92 @@ lemma tick_2: "Common.tick common = common' \<Longrightarrow> Common.toList comm
 
 lemma pop: "\<lbrakk>\<not> isEmpty common; pop common = (x, common')\<rbrakk> \<Longrightarrow> x # toList common' = toList common"
   apply(induction common arbitrary: x rule: pop.induct)
-  by(auto simp: get  split: prod.splits)
+   apply(auto simp: get  split: prod.splits current.splits if_splits)
+  using get by fastforce+
 
 lemma push: "toList (push x common) = x # toList common"
   apply(induction x common rule: push.induct)
   by(auto simp: put)
+
+lemma take_hd: "xs \<noteq> [] \<Longrightarrow> take (Suc 0) xs = [hd xs]"
+  apply(induction xs)
+  by auto
+
+lemma invariant_tick: "invariant common \<Longrightarrow> invariant (tick common)" 
+  apply(induction common rule: tick.induct)
+   apply(auto split: current.splits)
+    (* TODO: *)
+  apply (metis Suc_diff_Suc append_Nil diff_is_0_eq' nat_neq_iff rev_append rev_rev_ident size_listLength take_Nil take_hd)
+    by (metis Suc_diff_Suc gen_length_def hd_Cons_tl hd_take le_SucI length_append length_code length_rev list.size(3) nat_le_linear not_le rev.simps(2) size_listLength take_tl zero_less_Suc)
+
+lemma invariant_push: "invariant common \<Longrightarrow> invariant (push x common)"
+  apply(induction x common rule: push.induct)
+  by(auto simp: invariant_put size_push put Stack_Proof.push split: current.splits)
+
+(* TODO: *)
+
+lemma helper_2: "n < length xs \<Longrightarrow> tl (rev (take (Suc n) xs)) = rev (take n xs)"
+  apply(induction xs; induction n)
+     apply auto
+  by (metis Suc_diff_Suc drop_Suc gr_implies_not0 length_0_conv old.nat.distinct(2) rev_is_Nil_conv rev_take take_eq_Nil tl_append2 tl_drop)
+
+lemma helper_1: 
+assumes
+  "\<not> Stack.isEmpty old"
+  "Stack.toList old = rev (take (Stack.size old - length new) aux) @ new"
+  "length new < Stack.size old"
+  "common' = Copy (Current [] 0 (Stack.pop old) (Stack.size old - Suc 0)) aux new (length new)" 
+  "\<not> Stack.size old - Suc 0 \<le> length new"
+  "x = first old"
+  "extra' = []" 
+  "added' = 0" 
+  "old' = Stack.pop old"
+  "remaining' = Stack.size old - Suc 0"
+shows
+  "Stack.toList (Stack.pop old) = rev (take (Stack.size old - Suc (length new)) aux) @ new"
+proof -
+  from assms have tl: "Stack.toList (Stack.pop old) = tl (Stack.toList old)"
+    by(auto simp: Stack_Proof.pop)
   
+  with assms have "tl (rev (take (Stack.size old - length new) aux)) = 
+                       rev (take (Stack.size old - Suc (length new)) aux)"
+    by (smt (z3) Suc_diff_Suc Suc_le_lessD append_eq_conv_conj diff_le_self helper_2 length_drop length_rev length_rotate rev_take rotate_append size_listLength)
+
+  with assms tl have "tl (rev (take (Stack.size old - length new) aux) @ new) = 
+                       rev (take (Stack.size old - Suc (length new)) aux) @ new"
+    by (metis append_Nil nat_neq_iff size_listLength tl_append2)
+
+  with assms tl show ?thesis
+    by auto
+  
+qed
+
+lemma helper: 
+  assumes
+  "\<not> Current.isEmpty (Current extra (length extra) old (Stack.size old))"
+  "get (Current extra (length extra) old (Stack.size old)) = (x, Current extra' added' old' remaining')"
+  "Stack.toList old = rev (take (Stack.size old - length new) aux) @ new"
+  "length new < Stack.size old"
+  "common' = Copy (Current extra' added' old' remaining') aux new (length new)"
+  " \<not> remaining' \<le> length new"
+  shows 
+  "Stack.toList old' = rev (take (remaining' - length new) aux) @ new"
+  using assms apply(induction extra)
+  by(auto simp: helper_1)
+  
+
+lemma invariant_pop: "\<lbrakk>\<not> isEmpty common; invariant common; pop common = (x, common')\<rbrakk>
+   \<Longrightarrow> invariant common'"
+  apply(induction common arbitrary: x rule: pop.induct)
+   apply(auto simp:  invariant_get get Stack_Proof.pop size_pop empty not_empty split: prod.splits current.splits)
+    (* TODO: *)   
+         apply (metis Stack_Proof.pop get length_Cons list.sel(3) not_empty size_listLength zero_less_Suc)
+        apply (metis empty get list.discI size_pop)
+  apply (smt (verit, ccfv_threshold) Current.invariant.simps Current.isEmpty.elims(1) Current.toList.simps append_eq_append_conv current.simps(1) get get.simps(1) get.simps(2) invariant_get leD length_Cons not_less_eq_eq order_class.order.antisym prod.simps(1) self_append_conv2 size_listLength)
+    apply (meson Current.invariant.simps invariant_get)
+  apply (meson Current.invariant.simps invariant_get)
+    apply(simp add: helper)
+   apply (meson Current.invariant.simps invariant_get)
+  by (meson Current.invariant.simps invariant_get)
+
 end
