Current_Proof.thy
@@ -11,4 +11,13 @@ lemma get: "\<lbrakk>\<not> isEmpty current; get current = (x, current')\<rbrakk
   apply(induction current arbitrary: x rule: get.induct)
   by(auto simp: first_pop)
 
+lemma invariant_put: "invariant current \<Longrightarrow> invariant (put x current)"
+  apply(induction x current rule: put.induct)
+  by auto
+
+lemma invariant_get: "\<lbrakk>\<not> isEmpty current; invariant current; get current = (x, current')\<rbrakk>
+   \<Longrightarrow> invariant current'"
+  apply(induction current arbitrary: x rule: get.induct)
+  by(auto simp: size_pop)
+
 end
