Idle_Proof.thy
@@ -1,0 +1,15 @@
+theory Idle_Proof
+  imports Idle Stack_Proof
+begin
+
+lemma push: "toList (push x idle) = x # toList idle"
+  apply(induction idle arbitrary: x)
+  by(auto simp: Stack_Proof.push)
+
+lemma size_push: "size (push x idle) = Suc (size idle)"
+  apply(induction idle arbitrary: x)
+  by(auto simp: Stack_Proof.size_push)
+
+
+
+end
