Small_Proof.thy
@@ -6,4 +6,25 @@ lemma tick: "toList (tick state) = toList state"
   apply(induction state)
   by(auto simp: tick split: current.splits)
 
+lemma push: "x # toList small = toList (push x small)"
+  apply(induction x small rule: push.induct)
+  by(auto simp: push put)
+
+lemma pop: "\<lbrakk>\<not> isEmpty small; pop small = (x, small')\<rbrakk> \<Longrightarrow> x # toList small' = toList small"
+  apply(induction small arbitrary: x rule: pop.induct)
+  by(auto simp: get Common_Proof.pop split: prod.splits current.splits if_splits)
+
+lemma invariant_tick: "invariant state \<Longrightarrow> invariant (tick state)"
+  quickcheck
+  sorry
+
+value "tick (Reverse2 (Current [] 0 (Stack [] [a\<^sub>1]) 1) [a\<^sub>1] (Stack [] []) [a\<^sub>2] 1)"
+
+lemma invariant_push: "invariant small \<Longrightarrow> invariant (push x small)"
+  sorry
+
+lemma invariant_pop: "\<lbrakk>\<not> isEmpty small; invariant small; pop_invariant small; pop small = (x, small')\<rbrakk>
+   \<Longrightarrow> invariant small'"
+  sorry
+
 end
