Transformation_Proof.thy
@@ -1,29 +1,73 @@
 theory Transformation_Proof
-  imports Transformation Small_Proof Big_Proof Stack_Proof Current_Proof
+  imports Transformation Small_Proof Big_Proof Stack_Proof Current_Proof 
 begin
 
 lemmas tick = Small_Proof.tick Big_Proof.tick Common_Proof.tick
 
 (* TODO: Naming *)
-lemma ticks_help: "ticksHelper (big, small) = (newBig, newSmall) \<Longrightarrow> Big.toList big = Big.toList newBig"
-  apply(induction "(big, small)" rule: ticksHelper.induct)
+lemma ticks_help: "tickStates (big, small) = (newBig, newSmall) \<Longrightarrow> Big.toList big = Big.toList newBig"
+  apply(induction "(big, small)" rule: tickStates.induct)
   by(auto simp: tick split: current.splits if_splits)
 
-lemma ticks_help2: "ticksHelper (big, small) = (newBig, newSmall) \<Longrightarrow> Small.toList small = Small.toList newSmall"
-  apply(induction "(big, small)" rule: ticksHelper.induct)
+lemma ticks_help2: "tickStates (big, small) = (newBig, newSmall) \<Longrightarrow> Small.toList small = Small.toList newSmall"
+  apply(induction "(big, small)" rule: tickStates.induct)
   by(auto simp: tick split: current.splits if_splits)
+
+lemma ticks_help': "tickStates (tickStates (tickStates (tickStates (big, small))))
+         = (newBig, newSmall) \<Longrightarrow> Big.toList big = Big.toList newBig"
+  by (metis prod.exhaust_sel ticks_help)
+
+lemma ticks_help2': "tickStates (tickStates (tickStates (tickStates  (big, small))))
+     = (newBig, newSmall) \<Longrightarrow> Small.toList small = Small.toList newSmall"
+  by (metis prod.exhaust_sel ticks_help2)
+
+
+lemma ticks_helpFUCK: "tickStates (big, push x small) = (newBig, newSmall) \<Longrightarrow> x #  Small.toList small = Small.toList newSmall"
+  apply(induction "(big, push x small)" rule: tickStates.induct)
+  by(auto simp: Small_Proof.push ticks_help2 split: current.splits if_splits)
+
+lemma fourTicks_helpFUCK: "tickStates (tickStates (tickStates (tickStates (big, push x small)))) = (newBig, newSmall) \<Longrightarrow> x #  Small.toList small = Small.toList newSmall"
+  by (simp add: Small_Proof.push ticks_help2')
+
+lemma ticks_helpFUCK': "tickStates (Big.push x big, small) = (newBig, newSmall) \<Longrightarrow> x # Big.toList big = Big.toList newBig"
+  apply(induction "(Big.push x big, small)" rule: tickStates.induct)
+      apply (smt (verit) Big.push.elims Big.state.simps Big.toList.simps put ticks_help)
+     apply (smt (verit) Big.push.elims Big.state.simps(4) Big.toList.simps(2) put ticks_help)
+  
+  apply (smt (verit) Big.push.elims Big.state.simps(4) Big.toList.simps(1) Common_Proof.push ticks_help)
+
+   apply (smt (verit, best) Big.push.elims Big.toList.simps(1) Big.toList.simps(2) Common_Proof.push put ticks_help)
+  by (smt (verit, best) Big.push.elims Big.toList.simps(1) Big.toList.simps(2) Common_Proof.push put ticks_help)
+
+lemma fourTicks_helpFUCK': "tickStates (tickStates (tickStates (tickStates (Big.push x big, small)))) = (newBig, newSmall) \<Longrightarrow> x # Big.toList big = Big.toList newBig"
+  by (metis prod.exhaust_sel ticks_help ticks_helpFUCK')
+  
+lemma ticks_helpFUCK_2: "tickStates (big, push x small) = (newBig, push y newSmall) \<Longrightarrow> Small.toList small = Small.toList newSmall"
+  apply(induction "(big, push x small)" rule: tickStates.induct)
+      apply(auto simp: tick push put split: current.splits if_splits)
+      apply (metis Small_Proof.push list.inject ticks_helpFUCK)
+     apply (metis Small_Proof.push Small_Proof.tick list.inject)
+    apply (metis Small_Proof.push Small_Proof.tick list.inject)
+   apply (metis Small_Proof.push list.inject ticks_helpFUCK)
+  by (metis Small_Proof.push list.inject ticks_helpFUCK)
 
 lemma ticks: "toListLeft (ticks transformation) = toListLeft transformation"
   apply(induction transformation rule: toListLeft.induct)
   by(auto simp: ticks_help ticks_help2 split: prod.splits)
 
-lemmas all_ticks = tick ticks
+lemma fourTicks: "toListLeft (fourTicks transformation) = toListLeft transformation"
+  by(auto simp: ticks)
+
+lemma sixTicks: "toListLeft (sixTicks transformation) = toListLeft transformation"
+  by(auto simp: ticks)
+
+lemmas all_ticks = tick ticks sixTicks fourTicks
 
 lemmas state_splits = idle.splits Common.state.splits Small.state.splits Big.state.splits
 
 (* TODO: *)
 lemma ticks_helper: "\<lbrakk>
-  ticksHelper
+  tickStates
          (Reverse (Current [] 0 (Stack.push x leftValues) (Stack.size leftValues - Stack.size rightValues)) (Stack.push x leftValues) [] (Stack.size leftValues - Stack.size rightValues),
          Reverse1 (Current [] 0 rightValues (Suc (2 * Stack.size rightValues))) rightValues []) = (left, right)
     \<rbrakk>
@@ -31,7 +75,7 @@ lemma ticks_helper: "\<lbrakk>
 proof(induction  
          "(Reverse (Current [] 0 (Stack.push x leftValues) (Stack.size leftValues - Stack.size rightValues)) (Stack.push x leftValues) [] (Stack.size leftValues - Stack.size rightValues)
          , Reverse1 (Current [] 0 rightValues (Suc (2 * Stack.size rightValues))) rightValues [])"
-        rule: ticksHelper.induct
+        rule: tickStates.induct
         )
   case 1
   then show ?case 
@@ -39,13 +83,12 @@ proof(induction
 next
   case ("2_1" vd)
    then have left: "left = Big.tick (Reverse (Current [] 0 (Stack.push x leftValues) (Stack.size leftValues - Stack.size rightValues)) (Stack.push x leftValues) [] (Stack.size leftValues - Stack.size rightValues))"
-     by (metis ticksHelper.simps(2) prod.inject)
+     by (metis tickStates.simps(2) prod.inject)
    then have right: "right = Small.tick (Reverse1 (Current [] 0 rightValues (Suc (2 * Stack.size rightValues))) rightValues [])"
-     by (metis "2_1.hyps" "2_1.prems" ticksHelper.simps(2) old.prod.inject)
+     by (metis "2_1.hyps" "2_1.prems" tickStates.simps(2) old.prod.inject)
    from left right show ?case
-     by(auto simp: Stack_Proof.push split: if_splits)
+     by (simp add: Big_Proof.tick Stack_Proof.push)
  qed
-
 
 lemma test_2_1: "put x current = Current x1 x2 x3 x4 
         \<Longrightarrow> x1 @ Stack.toList x3 = x # Current.toList current"
@@ -60,118 +103,16 @@ lemma small_push_2: "Small.toList (Small.push x small) = x # Small.toList small"
   apply(induction x small rule: Small.push.induct)
   by(auto simp: Common_Proof.push put)
 
-lemma test_2: "ticksHelper (big, Small.push x small) = (big', small')
+lemma test_2: "tickStates (big, Small.push x small) = (big', small')
            \<Longrightarrow> Small.toList small' = x # Small.toList small"
   by(auto simp: small_push ticks_help2)
 
-
 lemma test: " \<lbrakk>
-    ticksHelper (x1b, x2b) = (x1c, small'); 
-    ticksHelper (x1a, x2a) = (x1b, x2b); 
-    ticksHelper (x1, x2) = (x1a, x2a);
-    ticksHelper (right, Small.push x left) = (x1, x2)\<rbrakk>
+    tickStates (x1b, x2b) = (x1c, small'); 
+    tickStates (x1a, x2a) = (x1b, x2b); 
+    tickStates (x1, x2) = (x1a, x2a);
+    tickStates (right, Small.push x left) = (x1, x2)\<rbrakk>
        \<Longrightarrow> Small.toList small' = x # Small.toList left"
   by (metis ticks_help2 test_2)
-
-
-(*lemma something_1_1: "\<lbrakk>
-      ticksHelper (right, Small.push x left) = (Big.state.Common (state.Idle x21a (idle.Idle x1e x2f)), Small.state.Common (state.Idle x21 (idle.Idle x1d x2d)))
-    \<rbrakk> \<Longrightarrow> Stack.toList x1d  = x # Small.toList left"
-  sorry*)
-(* lemma something_1_2: "\<lbrakk>ticksHelper (ticksHelper (ticksHelper (ticksHelper (Reverse currentB big auxB 0, Small.push x left)))) =
-        (Big.state.Common (state.Idle x21a (idle.Idle x1e x2f)), Small.state.Common (state.Idle x21 (idle.Idle x1d x2d)))\<rbrakk>
-       \<Longrightarrow> Stack.toList x1d @ rev (Stack.toList x1e) = x # Small.toList left @ rev (Current.toList x21a)"
-  sorry
-
-lemma something_1_1: "\<lbrakk>
-      ticksHelper (right, Small.push x left) = (Big.state.Common (state.Idle x21a (idle.Idle x1e x2f)), Small.state.Common (state.Idle x21 (idle.Idle x1d x2d)))
-    \<rbrakk> \<Longrightarrow> Stack.toList x1d @ rev (Stack.toList x1e) = x # Small.toList left @ rev (Current.toList x21a)"
- 
-  sorry
-
-lemma something_now: "ticksHelper(ticksHelper(ticksHelper(ticksHelper(big, small)))) = (newBig, newSmall) \<Longrightarrow> 
-    Small.toList newSmall @ rev (Big.toList newBig) = Small.toList small @ rev (Big.toList big)"
-  by (metis old.prod.exhaust ticks_help ticks_help2)
-
-
-lemma something_1: "\<lbrakk>
-      ticksHelper(ticksHelper(ticksHelper(ticksHelper (right, Small.push x left)))) = (Big.state.Common (state.Idle x21a (idle.Idle x1e x2f)), Small.state.Common (state.Idle x21 (idle.Idle x1d x2d)))
-    \<rbrakk> \<Longrightarrow> Stack.toList x1d @ rev (Stack.toList x1e) = x # Small.toList left @ rev (Current.toList x21a)"
-  apply(induction x left arbitrary: right x2f x2d rule: Small.push.induct)
-  apply(auto simp: something_now split: if_splits current.splits)
-  sorry
-
-lemma something: " \<lbrakk>
-        ticksHelper (x1b, x2b) = (Big.state.Common (state.Idle x21a (idle.Idle x1e x2f)), Small.state.Common (state.Idle x21 (idle.Idle x1d x2d)));
-        ticksHelper (x1a, x2a) = (x1b, x2b); 
-        ticksHelper (x1, x2) = (x1a, x2a); 
-      ticksHelper (right, Small.push x left) = (x1, x2)
-    \<rbrakk> \<Longrightarrow> Stack.toList x1d @ rev (Stack.toList x1e) = x # Small.toList left @ rev (Current.toList x21a)"
-  by (metis something_1) *)
-
-(*
-lemma test1_1_1: "put x r1 = Current r1' r2' r3' r4' \<Longrightarrow> r1' @ Stack.toList r3' = x # Current.toList r1"
-  apply(induction r1 rule: Current.toList.induct)
-  by auto
-
-lemma test1_1: "
-       ticksHelper (Reverse l1 l2 l3 l4) (Reverse1 (put x r1) r2 r3) =
-       (Reverse l1' l2' l3' l4', Reverse1 (Current r1' r2' r3' r4') small auxS) \<Longrightarrow>
-       r1' @ Stack.toList r3' @ rev (Current.toList l1') = x # Current.toList r1 @ rev (Current.toList l1)"
-  apply(induction "Reverse l1 l2 l3 l4" "Reverse1 (put x r1) r2 r3" rule: ticksHelper.induct)
-  by(auto simp: test1_1_1 split: if_splits)
-
-lemma test1_2: "\<lbrakk>
-    put x current = Current extra added old remained
-  \<rbrakk> \<Longrightarrow> extra @ Stack.toList old @ rev (Common.toList (Common.tick common)) = x # Current.toList current @ rev (Common.toList common)"
-  apply(induction current rule: Current.toList.induct)
-  by(auto simp: tick)
-
-lemma test1_3: "
-      ticksHelper (Reverse x1 x2aa x3 x4) (Reverse1 (put xa x1aa) x2 x3aa) = 
-      (Big.state.Common x, Reverse1 (Current x1a x2a x3a x4a) small auxS)
-       \<Longrightarrow>
-      x1a @ Stack.toList x3a @ rev (Common.toList x) = xa # Current.toList x1aa @ rev (Current.toList x1)"
-  apply(induction "Reverse x1 x2aa x3 x4" "Reverse1 (put xa x1aa) x2 x3aa" rule: ticksHelper.induct)
-  by auto
-
-lemma test1: "\<lbrakk>
-  ticksHelper right (Small.push x left) = (big, Reverse1 current small auxS)
-  \<rbrakk> \<Longrightarrow> Current.toList current @ rev (Big.toList big) = x # Small.toList left @ rev (Big.toList right)"
-  apply(induction left; induction right; induction big; induction current arbitrary: x small auxS)
-  by(auto simp: test1_1 test1_2 test1_3 split: if_splits)
-
-lemma test2_1: "\<lbrakk>
-  Reverse1 currentS uu auxS = Small.push x left;
-  Small.tick right = Reverse1 x11 x12 x13;
-  ticksHelper (Reverse currentB big auxB 0) (Small.push x left) = (Reverse v va vb (Suc vd), right)
-  \<rbrakk> \<Longrightarrow> Current.toList x11 @ rev (Current.toList v) = x # Small.toList left @ rev (Current.toList currentB)"
-  apply(induction "Reverse currentB big auxB 0" "Small.push x left" rule: ticksHelper.induct;
-        induction x11 rule: Current.toList.induct;
-        induction currentB rule: Current.toList.induct;
-        induction left rule: Small.toList.induct;
-        induction v arbitrary: x rule: Current.toList.induct)
-  by auto
-
-lemma test2: "\<lbrakk>
-  ticksHelper x1 x2 = (x1c, Reverse1 x11 x12 x13); 
-  ticksHelper right (Small.push x left) = (x1, x2)
-  \<rbrakk> \<Longrightarrow> Current.toList x11 @ rev (Big.toList x1c) = x # Small.toList left @ rev (Big.toList right)"
-  apply(induction right "Small.push x left" rule: ticksHelper.induct;
-        induction x1 x2 arbitrary: x left x11 x12 x13 x1c  rule: ticksHelper.induct)
-   apply(auto simp: test2_1 split: if_splits)
-  sorry
-
-lemma test: "\<lbrakk>
-  ticksHelper x1b x2b = (x1c, Reverse1 x11 x12 x13); 
-  ticksHelper x1a x2a = (x1b, x2b); 
-  ticksHelper x1 x2 = (x1a, x2a);
-  ticksHelper right (Small.push x left) = (x1, x2)
-  \<rbrakk> \<Longrightarrow> Current.toList x11 @ rev (Big.toList x1c) = x # Small.toList left @ rev (Big.toList right)"
-  apply(auto simp: ticks_help ticks_help2)
-(*apply(induction right "Small.push x left" rule: ticksHelper.induct;
-        induction x1 x2 rule: ticksHelper.induct;
-        induction x1a x2a rule: ticksHelper.induct)*)
-  sorry*)
 
 end
